Update history

history.fst
@@ -1,8 +1,8 @@
 module History
 
-open FStar.Tactics
-module T = FStar.Tactics
-open FStar.Tactics.Typeclasses
+//open FStar.Tactics
+//module T = FStar.Tactics
+//open FStar.Tactics.Typeclasses
 
 module L = FStar.List.Tot
 
@@ -61,11 +61,87 @@ val hbeq_reflexive : #s:eqtype -> #o:eqtype -> h:history s o
                    -> Lemma (ensures (hbeq h h))
 let hbeq_reflexive h = ()
 
-val lemma1 : #s:eqtype -> #o:eqtype -> {| M.mrdt s o |} -> h:history s o{wellformed h}
-           -> Lemma (ensures (forall h'. hbeq h h' ==> wellformed h'))  (decreases (size h))
+val lemma1 : #s:eqtype -> #o:eqtype -> {| M.mrdt s o |} 
+           -> h:history s o{wellformed h}
+           -> Lemma (ensures (forall h'. hbeq h h' ==> wellformed h')) (decreases (size h))
 let rec lemma1 (History s ch) = 
   match ch with
   | [] -> ()
   | (_,x)::xs -> 
      lemma1 x; 
      lemma1 (History s xs)
+
+val concurrent_list : #s:eqtype -> #o:eqtype 
+                    -> h:history s o 
+                    -> l:list (history s o) 
+                    -> r:bool{(forall h'. L.mem h' l ==> concurrent h h') <==> r = true}
+let rec concurrent_list h l =
+  match l with
+  | [] -> true
+  | x::xs -> concurrent h x && concurrent_list h xs
+
+val cross_concurrent : #s:eqtype -> #o:eqtype
+                     -> l:list (history s o)
+                     -> r:list (history s o){(forall c. L.mem c r ==> L.mem c l) /\
+                                            (forall c1 c2. L.mem c1 r /\ L.mem c2 r /\ ~(c1 = c2) ==> concurrent c1 c2)}
+let rec cross_concurrent l = 
+  match l with
+  | [] -> []
+  | x::xs -> 
+      if concurrent_list x xs then 
+        x::cross_concurrent xs
+      else cross_concurrent xs
+
+val append : #s:eqtype -> #o:eqtype -> p:(history s o -> bool) 
+           -> l1:list (history s o){forall e. L.mem e l1 ==> p e}
+           -> l2:list (history s o){forall e. L.mem e l2 ==> p e}
+           -> l:list (history s o){forall e. L.mem e l ==> p e}
+let rec append p l1 l2 =
+  match l1 with
+  | [] -> l2
+  | x::xs -> x::(append p xs l2)
+
+val lca_ : #s:eqtype -> #o:eqtype //-> {| M.mrdt s o |} XXX KC TODO
+        -> m:M.mrdt s o
+        -> h:history s o
+        -> a:history s o{hb h a}
+        -> b:history s o{hb h b}
+        -> Tot (lcalst: list (history s o){(forall l. L.mem l lcalst ==> hb h l /\ hbeq l a /\ hbeq l b) /\ 
+                                          (forall l1 l2. L.mem l1 lcalst /\ L.mem l2 lcalst /\ ~(l1 = l2) ==> concurrent l1 l2)})
+              (decreases (size h))
+let rec lca_ m h a b =
+  let History s ch = h in
+  match ch with
+  | [] -> []
+  | (_,x)::xs ->
+      let l1 =
+        if hb x a && hb x b then
+          lca_ m x a b
+        else []
+      in
+      let h' = History s xs in
+      let l2 = 
+        if hb h' a && hb h' b then
+          lca_ m h' a b
+        else []
+      in
+      assert (forall c. L.mem c l1 ==> hbeq c a /\ hbeq c b);
+      assert (forall c. L.mem c l2 ==> hbeq c a /\ hbeq c b);
+      let p = fun c -> hb h c && hbeq c a && hbeq c b in
+      let l = (append p l1 l2) in
+      cross_concurrent l
+
+val lca : #s:eqtype -> #o:eqtype //-> {| M.mrdt s o |} XXX KC TODO
+        -> m:M.mrdt s o
+        -> h:history s o
+        -> a:history s o{hbeq h a}
+        -> b:history s o{hbeq h b}
+        -> Tot (lcalst: list (history s o){(forall l. L.mem l lcalst ==> hbeq h l /\ hbeq l a /\ hbeq l b) /\ 
+                                          (forall l1 l2. L.mem l1 lcalst /\ L.mem l2 lcalst /\ ~(l1 = l2) ==> concurrent l1 l2)})
+              (decreases (size h))
+let lca m h a b = 
+  if h = a || h = b then [h]
+  else begin
+    assert (hb h a /\ hb h b);
+    cross_concurrent (h::lca_ m h a b)
+  end
